src/openflow_controller.ml
@@ -4,6 +4,7 @@ open Async.Std
 let logical_or = Int32.logor
 let int32_to_int = Int32.to_int
 let int64_to_int = Int64.to_int
+let int_to_int64 = Int64.of_int
 let nth = List.nth
 
 open Core.Std
@@ -19,18 +20,17 @@ let rec word_to_int32 w = match w with
       then Int32.succ (Int32.shift_left (word_to_int32 w') 1)
       else Int32.shift_left (word_to_int32 w') 1
 
-let ip_to_mask ip =
-  let int32_rep = logical_or
-    (logical_or
-      (Int32.shift_left (word_to_int32 (fst (fst (fst ip)))) 24)
-      (Int32.shift_left (word_to_int32 (snd (fst (fst ip)))) 16)
-    )
-    (logical_or
-      (Int32.shift_left (word_to_int32 (snd (fst ip))) 8)
-      (word_to_int32 (snd ip))
-    )
-  in
-    { m_value = int32_rep; m_mask = None }
+let ip_to_int32 ip = logical_or
+  (logical_or
+    (Int32.shift_left (word_to_int32 (fst (fst (fst ip)))) 24)
+    (Int32.shift_left (word_to_int32 (snd (fst (fst ip)))) 16)
+  )
+  (logical_or
+    (Int32.shift_left (word_to_int32 (snd (fst ip))) 8)
+    (word_to_int32 (snd ip))
+  )
+
+let ip_to_mask ip = { m_value = ip_to_int32 ip; m_mask = None }
 
 let generate_flow_mod_message entry = FlowModMsg {
   command = AddFlow;
@@ -61,20 +61,36 @@ let generate_flow_mod_message entry = FlowModMsg {
     | Drop -> []
 }
 
+let delete_all_flows_message = FlowModMsg {
+  command = DeleteFlow;
+  priority = 99;
+  cookie = 0L;
+  idle_timeout = Permanent;
+  hard_timeout = Permanent;
+  notify_when_removed = false;
+  apply_to_packet = None;
+  out_port = None;
+  check_overlap = false;
+  pattern = match_all;
+  actions = []
+}
+
+let find_node_with_ip ip32 = List.find all_nodes (fun node -> ip_to_int32 (node_ips node) = ip32)
+
 (* Note: This requires the user to arrange switch IDs in the same order as their Coq inductive type
  * i.e. the first switch has ID 1, second has ID 2, etc. *)
 let switch_id_to_node sw_id = nth all_nodes (int64_to_int sw_id - 1)
 
-let switch (ctl : Async_OpenFlow.OpenFlow0x01.Controller.t) _ evt =
+let switch (ctl : Async_OpenFlow.OpenFlow0x01.Controller.t) (state : (exampleVertex * exampleVertex) list) evt =
   match evt with
     | `Connect (sw_id, _) ->
       Deferred.all (
-        List.map (generated_controller_entries (switch_id_to_node sw_id)) (fun entry ->
+        List.map (generated_dynamic_controller.controller_state_decider state (switch_id_to_node sw_id)) (fun entry ->
           Async_OpenFlow.OpenFlow0x01.Controller.send ctl sw_id (1l, generate_flow_mod_message entry)
         )
-      )
+      ) >>= (fun _ -> return state)
     | `Disconnect (_, _) ->
-      return []
+      return state
     | `Message (sw_id, (_xid, msg)) ->
       match msg with
       | PacketInMsg pktIn ->
@@ -85,23 +101,41 @@ let switch (ctl : Async_OpenFlow.OpenFlow0x01.Controller.t) _ evt =
             (packetIn_to_string pktIn)
         );
         if pktIn.reason = ExplicitSend
-        then ((* TODO: resend all flows *))
-        else ();
-        return []
+        then
+          let packet = parse_payload pktIn.input_payload
+          in let maybe_src_node = find_node_with_ip (Packet.nwSrc packet)
+          in let maybe_dest_node = find_node_with_ip (Packet.nwDst packet)
+          in match maybe_src_node, maybe_dest_node with
+          | Some src_node, Some dest_node ->
+            let processed_flow = { src = src_node; dest = dest_node }
+            in let new_state = generated_dynamic_controller.controller_system.step state processed_flow
+            in Deferred.all (
+              List.mapi all_nodes (fun index node ->
+                let dest_switch_id = int_to_int64 (index + 1)
+                in (Async_OpenFlow.OpenFlow0x01.Controller.send ctl dest_switch_id (1l, delete_all_flows_message)
+                  >>= fun _ -> Deferred.all (
+                    List.map (generated_dynamic_controller.controller_state_decider new_state node) (fun entry ->
+                      Async_OpenFlow.OpenFlow0x01.Controller.send ctl dest_switch_id (1l, generate_flow_mod_message entry)
+                    )
+                  )
+                )
+              )
+            ) >>= (fun _ -> print_endline "sent new flows"; return new_state)
+          | _, _ -> return state
+        else return state
       | ErrorMsg err ->
         print_endline "error message";
-        return []
+        return state
       | PortStatusMsg ps ->
-        print_endline "port status";
-        return []
+        return state
       | _ ->
         print_endline "other";
-        return []
+        return state
 
 let main () =
   Async_OpenFlow.OpenFlow0x01.Controller.create 6633 () >>=
     fun t ->
-      Pipe.fold (Async_OpenFlow.OpenFlow0x01.Controller.listen t) ~init:[] ~f:(switch t)
+      Pipe.fold (Async_OpenFlow.OpenFlow0x01.Controller.listen t) ~init:(generated_dynamic_controller.controller_system.initial) ~f:(switch t)
 
 let _ = main ()
 let _ = never_returns (Scheduler.go ())
